

FYS4480/9480, lecture  
November 20, 2025

# FYS4480/9480 November 20

FC1

$$\mathcal{H}|\psi_0\rangle = E_0|\psi_0\rangle$$

$$|\psi_0\rangle = (1 + \hat{C})|\Phi_0\rangle$$

$$\mathcal{H}_0|\Phi_0\rangle = E_0|\Phi_0\rangle$$

$$\Delta E_0 = E_0 - E_0^{\text{Ref}}$$

$$E_0^{\text{Ref}} = \langle \Phi_0 | \mathcal{H} | \Phi_0 \rangle$$

$$\hat{C} = \sum_{p_H > 0} c_H^p \hat{A}_H^p |\Phi_0\rangle$$

$$\hat{A}_H^p = a_a^\dagger a_b^\dagger \dots a_{i_1} \dots a_{j_1} a_{i_2} \dots a_{j_2} \dots$$

$$|4_0\rangle = \exp\left\{\hat{T}\right\} | \Phi_0 \rangle$$

$$\hat{T} = \underbrace{\hat{T}_1}_{1p1h} + \underbrace{\hat{T}_2}_{2p2h} - \dots - \hat{T}_{npnh}$$

$$\underbrace{\hat{T}_1}_{1p1h} = \sum_{ai} a_a^\dagger a_i \tau_a^a$$

↑ unknown amplitudes

$$\underbrace{\hat{T}_2}_{2p2h} = \frac{1}{4} \sum_{abij} \tau_{ij}^{ab} \underbrace{(a_a^\dagger a_i)(a_b^\dagger a_j)}_{a_a^\dagger a_b^\dagger a_j a_i}$$

$$|\psi_0\rangle = e^T |\Phi_0\rangle$$

$$\mathcal{H} e^T |\Phi_0\rangle = E_0 e^T |\Phi_0\rangle$$

$$e^{-T} \mathcal{H} e^T |\Phi_0\rangle = E_0 |\Phi_0\rangle$$

$$\mathcal{H} = \mathcal{H}_N + E_0^{\text{ref}}$$

$$\underbrace{e^{-T} \mathcal{H}_N e^T}_{\text{onebody}} |\Phi_0\rangle = \Delta E_0 |\Phi_0\rangle$$

$$\mathcal{H}_N = \underbrace{\hat{T}_N}_{\text{onebody}} + \underbrace{\hat{V}_N}_{\text{twobody}}$$

Look back at FCI

$$\mathcal{H}|\psi_0\rangle = E_0|\psi_0\rangle$$

$$\mathcal{H} \sum_{PH} C_H^P |\Phi_H^P\rangle$$

$$\left\{ |\Phi_H^P\rangle = A_H^P |\Phi_H\rangle \right.$$

$$\langle \Phi_0 | \mathcal{H} | \psi_0 \rangle = E_0 \sum_{PH} C_H^P \langle \Phi_0 | \Phi_H^P \rangle$$

$$\begin{bmatrix} H_{00} & H_{01} & \dots & H_{0NPH} \\ H_{10} & & & \\ \vdots & & & \\ H_{NPH0} & & & \end{bmatrix} \begin{bmatrix} C_0 \\ C_1 \\ \vdots \\ C_{NPH} \end{bmatrix}$$

$H_{NPHNPH}$

$$\langle \Phi_0 | \mathcal{H} \sum_{\mathcal{PH}} C_{\#}^{\mathcal{P}} | \Phi_{\#}^{\mathcal{P}} \rangle = \langle \Phi_0 | E_0 | \sum_{\mathcal{P}, \#} C_{\#}^{\mathcal{P}}$$

$$C_0 = \underline{1} \quad \times | \Phi_{\#}^{\mathcal{P}} \rangle$$

$$\langle \Phi_0 | \mathcal{H} | \Phi_0 \rangle + \sum_{a_i} C_i^a \langle \Phi_0 | \mathcal{H} | \Phi_i^a \rangle$$

$$+ \sum_{\substack{ab \\ ij}} C_{ij}^{ab} \langle \Phi_0 | \mathcal{H} | \Phi_{ij}^{ab} \rangle = E_0$$

$$E_0^{\mathcal{H}E} + \sum_{a_i} C_i^a \langle i | f | a \rangle + \sum_{\substack{ab \\ ij}} C_{ij}^{ab} \langle ab | v | ij \rangle_{AS} = E_0$$

$$\Delta E_0 = E_0 - E_0^{\text{Ref}} =$$

$$\sum_{a,i} C_i^a \langle i | f | a \rangle + \sum_{\substack{i,j \\ a,b}} C_{ij}^{ab} \langle ab | v | ij \rangle$$

$$\langle \Phi_n^a | \mathcal{H} \sum_{PH} C_H^P | \Phi_H^P \rangle$$

$$= \langle \Phi_n^a | E_0 | \sum_{PH} C_H^P | \Phi_H^P \rangle$$

$$= E_0 C_n^a$$

$$= \langle \Phi_n^a | \mathcal{H} | \Phi_0 \rangle$$

$$+ \sum_{b_j'} C_j^b \langle \Phi_n^a | \mathcal{H} | \Phi_j^b \rangle$$

$$+ \sum_{\substack{bc \\ jk}} C_{jk}^{bc} \langle \Phi_n^a | \mathcal{H} | \Phi_{jk}^{bc} \rangle$$

$$+ \sum_{\substack{bcd \\ jk\ell}} C_{jk\ell}^{bcd} \langle \Phi_n^a | \mathcal{H} | \Phi_{jk\ell}^{bcd} \rangle$$



$$\langle \Phi_{ij}^{\alpha} | \mathcal{H} \sum_{PH} C_H^P | \Phi_H^P \rangle = E_0 C_{ij}^{\alpha}$$

$$\langle a e | v | r_j \rangle$$

$$\langle \Phi_{ij}^{\alpha} | \mathcal{H} | \Phi_0 \rangle + \sum_{ck} C_k^c \langle \Phi_{ij}^{\alpha} | \mathcal{H}$$

$$\times | \Phi_k^c \rangle + \sum_{ca} C_{ke}^{ca} \langle \Phi_{ij}^{\alpha} | \mathcal{H} | \Phi_{ke}^{ca} \rangle$$

$$+ \sum_{cde} C_{kcm}^{cde} \langle \Phi_{ij}^{\alpha} | \mathcal{H} | \Phi_{kcm}^{cde} \rangle$$

$$+ \sum_{cdef} C_{klmn}^{cdef} \langle - - - \rangle$$

CC theory

approx :  $T = T_2 = \frac{1}{4} \sum_{ij} t_{ij}^{ak}$

$[CCD, D = \text{doubler}]$   
 $= 2P24$

$$e^T |\Phi_0\rangle \approx e^{\overline{T}_2} |\Phi_0\rangle$$

$$\overline{T}_1 = 0 \quad \text{all } t_i^a = 0$$

$$H e^{\overline{T}_2} |\Phi_0\rangle = E_{CCD} e^{\overline{T}_2} |\Phi_0\rangle$$

$$\langle \Phi_0 | \text{ and } \langle \Phi_{ij}^{ak} |$$

$$e^{\overline{T}_2} = \left( 1 + \overline{T}_2 + \frac{1}{2!} \overline{T}_2^2 + \dots \right)$$

$$\langle \Phi_c | \mathcal{H} e^{\overline{T}_2} | \Phi_c \rangle = E_{\text{c.c.}} \langle \Phi_c | e^{\overline{T}_2} | \Phi_c \rangle$$

$$\langle \Phi_c | \mathcal{H} \left( 1 + \overline{T}_2 + \frac{1}{2!} \overline{T}_2^2 + \dots \right) | \Phi_c \rangle = E_0$$

$$\underbrace{\langle \Phi_c | \mathcal{H} | \Phi_0 \rangle}_{E_{\text{ref}}} + \langle \Phi_c | \mathcal{H} \overline{T}_2 | \Phi_0 \rangle = E_{\text{c.c.}}$$

$$\overline{T}_2^2 | \Phi_c \rangle \propto 4p4h \text{ stat.}$$

$$\langle \Phi_0 | \mathcal{H} T_2 | \Phi_0 \rangle = \Delta E_{\text{CCD}} = E_{\text{CCD}} - E_0^{\text{HF}}$$

$$\mathcal{H} = E_0^{\text{HF}} + \hat{T}_N + \hat{V}_N$$

$$\begin{aligned} \langle \Phi_0 | T_2 | \Phi_0 \rangle E_0^{\text{HF}} &+ \langle \Phi_0 | \hat{T}_N T_2 | \Phi_0 \rangle \\ &+ \langle \Phi_0 | \hat{V}_N T_2 | \Phi_0 \rangle \end{aligned}$$

$a_p^\dagger a_q$        $a_a^\dagger a_b^\dagger a_j a_{i'}$

$$\langle \Phi_0 | \underbrace{a_p^\dagger a_q a_a^\dagger a_b^\dagger}_{\text{red}} a_j a_{i'} | \Phi_0 \rangle$$

$$\langle \Phi_0 | V_N T_2 | \Phi_0 \rangle = \Delta E_{\text{CCD}}$$

$$= \left(\frac{1}{4}\right)^2 \sum_{\substack{pqrs \\ abij}} \langle \Phi_0 | \overbrace{a_p^\dagger a_q^\dagger a_r^\dagger a_s^\dagger}^{\delta_{st}} \underbrace{a_a^\dagger a_b^\dagger}_{\delta_{ab}} \underbrace{a_i a_j}_{\delta_{ji}} | \Phi_0 \rangle \times \langle pqrs | abij \rangle t_{ij}^{ab}$$

$$= \frac{1}{4} \sum_{\substack{ab \\ ij}} t_{ij}^{ab} \langle ij | ab \rangle = \Delta E_{\text{CCD}}$$

$= 0 \text{ with HF}$

$$\text{FCI} : \Delta E_0 = \sum_{ai} C_i^a \langle i | f_a \rangle + \sum_{\substack{ab \\ ij}} C_{ij}^{ab} \langle ij | ab \rangle$$

$$\langle \Phi_{ij}^{ab} | H e^{\overline{T}_2} | \Phi_c \rangle =$$

$$\langle \Phi_{ij}^{ab} | E_0 \left( 1 + \overline{T}_2 + \frac{\overline{T}_2^2}{2!} + \dots \right) | \Phi_c \rangle$$

$$= \langle \Phi_{ij}^{ab} | \overline{T}_2 | \Phi_c \rangle E_0$$

$$= \langle \Phi_0 | a_i^\dagger a_j^\dagger a_k a_a \frac{1}{4} \sum_{\substack{cd \\ kl}} t_{kl}^{ca}$$

$$a_c^\dagger a_d^\dagger a_e a_k | \Phi_0 \rangle \times$$

$$E_0$$



$$\langle \Phi_{ij}^{ab} | (F_N + V_N) (1 + T_2 + \frac{1}{2} T_2^2 + \dots) | \Phi_c \rangle$$

$$= (E_{\text{ccD}} - E_0^{\text{ref}}) t_{ij}^{ab} =$$

$$\Delta E_{\text{ccD}} t_{ij}^{ab}$$

$$\downarrow$$

$$\frac{1}{4} \sum_{\substack{cd \\ ke}} t_{ke}^{ca} \langle k e | v | c d \rangle$$

non-linear in  $t_{ij}^{ab}$   
(unknown)



$$\langle \Phi_{ij}^{ab} | (F_N + V_N) (1 + T_2 + \frac{1}{2} T_2^2 + \dots) | \Phi_0 \rangle$$

$$(i) \quad \langle \Phi_{ij}^{ab} | F_N | \Phi_0 \rangle = 0$$

$$(i') \quad \langle \Phi_{ij}^{ab} | F_N T_2 | \Phi_0 \rangle = ?$$

$$(i'') \quad \langle \Phi_{ij}^{ab} | F_N T_2^2 | \Phi_0 \rangle = 0$$

$$(iv) \quad \langle \Phi_{ij}^{ab} | V_N | \Phi_0 \rangle \neq 0$$

$$(v) \quad \langle \Phi_{ij}^{ab} | V_N T_2 | \Phi_0 \rangle \neq 0$$

$$(vi) \quad \langle \Phi_{ij}^{ab} | V_N T_2^2 | \Phi_0 \rangle \neq 0$$

$$F_N = \sum_{pq} \langle p | f | q \rangle a_p^\dagger a_q$$

$$\sum_{pq} \underbrace{\langle \Phi_{ij}^{cd} | a_p^\dagger a_q a_c^\dagger a_d^\dagger a_e a_k | \Phi_0 \rangle}_{\times t_{ke}^{cd}} \langle p | f | q \rangle \cdot \frac{1}{4}$$

$$\langle \Phi_0 | a_i^\dagger a_j^\dagger a_k a_l a_p^\dagger a_q^\dagger a_c^\dagger a_d^\dagger a_e a_k | \Phi_0 \rangle$$

$$\delta_{ik} \delta_{je} \delta_{ld} \delta_{ap} \delta_{qc}$$

$$\frac{1}{4} \sum_c \langle a | f | c \rangle t_{ij}^{cb}$$

$$a_i^\dagger a_j^\dagger a_b a_a a_p^\dagger a_q^\dagger a_c^\dagger a_d^\dagger a_e a_k$$

$$- \sum_l \langle l | f | j \rangle t_{ie}^{ab}$$

two more terms

$$- \sum_k \langle k | f | i \rangle t_{kj}^{ab}$$

$$+ \sum_a \langle b | f | a \rangle t_{ij}^{ad}$$